Changed Eq ctxmem and Luo_cut ID case works now

ECCA/core.v
@@ -30,8 +30,6 @@ Inductive exp {V: nat}: Type :=
   | eApp (v1 v2: exp)
   | eFst (v: exp)
   | eSnd (v: exp)
-  | eRefl (v: exp)
-  | eEqv (v1 v2: exp)
 .
 
 Hint Constructors exp.
@@ -66,8 +64,6 @@ Module ECCATerm <: Term.
       | eTru => eTru
       | eFls => eFls
       | eBool => eBool
-      | eRefl e => eRefl (kleisli f V e)
-      | eEqv e1 e2 => eEqv (kleisli f V e1) (kleisli f V e2)
       end.
 
   Lemma left_identity :
@@ -148,8 +144,6 @@ Fixpoint esize {V: nat} (e: @exp V) : nat :=
   | eTru => 1
   | eFls => 1
   | eBool => 1
-  | eRefl e => 1 + esize e
-  | eEqv e1 e2 => 1 + esize e1 + esize e2  
 end.
 
 Lemma esize_non_zero : forall V e, 0 < @esize V e.
@@ -190,8 +184,6 @@ Inductive Vclosed : @term 0 -> Set :=
   | vc_eApp (v1 v2: exp) : Vclosed v1 -> Vclosed v2 -> Vclosed (eApp v1 v2)
   | vc_eFst (v: exp) : Vclosed v -> Vclosed (eFst v)
   | vc_eSnd (v: exp) : Vclosed v -> Vclosed (eSnd v)
-  | vc_eRefl (v: exp): Vclosed v -> Vclosed (eRefl v)
-  | vc_eEqv (v1: exp) (v2: exp): Vclosed v1 -> Vclosed v2 -> Vclosed (eEqv v1 v2)
 .
 
 Check Vclosed_ind.
@@ -311,23 +303,6 @@ Fixpoint always_Vclosedk {V : nat} (t : term) {struct t} : Vclosedk V t :=
       | S V => fun _ vv a => go _ (vv a)
       end
     in go _ (always_Vclosedk v)
-  | eRefl v =>
-    let fix go {V} : forall v, Vclosedk V v ->
-                                 Vclosedk V (eRefl v) :=
-      match V with
-      | 0 => vc_eRefl
-      | S V => fun _ vv a => go _ (vv a)
-      end
-    in go _ (always_Vclosedk v)
-  | eEqv f e  =>
-    let fix go {V} : forall f e, Vclosedk V f ->
-                                 Vclosedk V e ->
-                                 Vclosedk V (eEqv f e) :=
-      match V with
-      | 0 => vc_eEqv
-      | S V => fun _ _ vf ve a => go _ _ (vf a) (ve a)
-      end
-    in go _ _ (always_Vclosedk f) (always_Vclosedk e)
 end.
 
 Definition term_ind
@@ -358,8 +333,6 @@ Definition term_ind
              (IFF : forall (v e1 e2 : exp), P v -> P e1 -> P e2 -> P (eIf v e1 e2))
              (FST : forall (v : exp), P v -> P (eFst v))
              (SND : forall (v : exp), P v -> P (eSnd v))
-             (RFL : forall (v : exp), P v -> P (eRefl v))
-             (EQV : forall (e1 e2 : exp), P e1 -> P e2 -> P (eEqv e1 e2))
              (tm : exp) : P tm :=
     Vclosed_ind (fun tm _ => P tm)
        IDD UNI
@@ -373,8 +346,6 @@ Definition term_ind
        (fun f e _ F _ E => APP f e F E)
        (fun v _ V => FST v V)
        (fun v _ V => SND v V)
-       (fun v _ V => RFL v V)
-       (fun e1 e2 _ E1 _ E2 => EQV e1 e2 E1 E2)
        tm (always_Vclosedk tm).
 
 Section term_ind_V.
@@ -406,10 +377,8 @@ Let PAIt := forall (v1 v2 A : exp), P v1 -> P v2 -> P A -> P (ePair v1 v2 A).
 Let IFFt := forall (v e1 e2 : exp), P v -> P e1 -> P e2 -> P (eIf v e1 e2).
 Let FSTt := forall (v : exp), P v -> P (eFst v).
 Let SNDt := forall (v : exp), P v -> P (eSnd v).
-Let RFLt := forall (v : exp), P v -> P (eRefl v).
-Let EQVt := forall (e1 e2 : exp), P e1 -> P e2 -> P (eEqv e1 e2).
 Variable (IDD: IDDt) (UNI: UNIt) (TRU: TRUt) (FLS: FLSt) (BOO: BOOt) (ABS: ABSt) (PIE: PIEt) (SIG: SIGt) (LET: LETt)
-(APP: APPt) (PAI: PAIt) (IFF: IFFt) (FST: FSTt) (SND: SNDt) (RFL: RFLt) (EQV: EQVt).
+(APP: APPt) (PAI: PAIt) (IFF: IFFt) (FST: FSTt) (SND: SNDt).
 Program Fixpoint term_ind_V
              (tm : exp) {measure (esize tm)}: P tm :=
 match tm with
@@ -427,8 +396,6 @@ match tm with
   | eApp v1 v2 => (APP _ _ (term_ind_V v1) (term_ind_V v2)) 
   | eFst v => FST _ (term_ind_V v)
   | eSnd v => SND _ (term_ind_V v)
-  | eRefl v => RFL _ (term_ind_V v)
-  | eEqv v1 v2 => EQV _ _ (term_ind_V v1) (term_ind_V v2)
 end.
 Solve All Obligations with (Tactics.program_simpl; try rewrite esize_open_id; cbn; lia).
 End term_ind_V.
@@ -497,13 +464,6 @@ with isVal {V}: exp -> Prop :=
   isConf A ->
   isConf B ->
   isVal (eSig A B)
-| Refl (v: exp):
-  isVal v ->
-  isVal (eRefl v)
-| Eqv (v1 v2: exp):
-  isVal v1 ->
-  isVal v2 ->
-  isVal (eEqv v1 v2)
 .
 Hint Constructors isConf isVal isComp.
 
@@ -561,13 +521,6 @@ Inductive squiv {V V1} : @exp V -> @exp V1 -> Prop:=
   | squivSnd (v v': exp):
     squiv v v' ->
     squiv (eSnd v) (eSnd v')
-  | squivRefl (v v': exp):
-    squiv v v' ->
-    squiv (eRefl v) (eRefl v')
-  | squivEqv (v1 v1' v2 v2': exp):
-    squiv v1 v1' ->
-    squiv v2 v2' ->
-    squiv (eEqv v1 v2) (eEqv v1' v2')
 .
 Hint Constructors squiv.
 
@@ -707,7 +660,7 @@ forall {V} {V'} (e: @exp V) (e': @exp V'), squiv e e' ->
 /\ (@isVal V e -> @isVal V' e')).
 Proof.
 intros. induction H; auto.
-1-4,10,11:repeat split; repeat destructConj; intros; constructANF; invertANF; auto.
+1-4:repeat split; repeat destructConj; intros; constructANF; invertANF; auto.
 1,2: repeat split; repeat destructConj; intros; try apply Let; invertANF; auto.
 + repeat split; repeat destructConj; intros. constructor; apply App; invertANF; auto.
   - apply App; invertANF; auto.
@@ -736,7 +689,7 @@ forall (V: nat),
 Proof.
 intros. cbn. apply val_conf_comp_comb; intros; unfold P in *; unfold P0 in *; unfold P1 in *.
 2,3,4,5: constructor.
-2,3,4,5,6,7,9,10,11,12,13: cbn; constructor; auto.
+2,3,4,5,6,7,9,10,11: cbn; constructor; auto.
 2,3: cbn; constructor; auto.
 apply renaming_ids_pANF. auto.
 Qed.
@@ -900,19 +853,10 @@ Let fAppT:=  (forall (v1 v2 : exp)
         P1 (eApp v1 v2) (App v1 v2 i i0)).
 Let fValT:= (forall (v : exp) (i : isVal v),
         P v i -> P1 v (ValIs v i)).
-Let fRflT:= (forall (v: exp) (i: isVal v),
-    P v i -> P (eRefl v) (Refl v i)).
-Let fEqvT:=  (forall (v1 v2 : exp)
-          (i : isVal v1),
-        P v1 i ->
-        forall (i0 : isVal v2),
-        P v2 i0 ->
-        P (eEqv v1 v2) (Eqv v1 v2 i i0)).
 
 Variable (fId: fIdT) (fTru: fTruT) (fFls: fFlsT) (fBool: fBoolT) (fUni: fUniT) (fPair: fPairT) (fPi: fPiT) (fAbs: fAbsT) (fSig: fSigT)
         (fLet: fLetT) (fIf: fIfT) (fComp: fCompT)
-        (fFst: fFstT) (fSnd: fSndT) (fApp: fAppT) (fVal: fValT)
-        (fRfl: fRflT) (fEqv: fEqvT).
+        (fFst: fFstT) (fSnd: fSndT) (fApp: fAppT) (fVal: fValT).
 
 Definition ANF_val_conf_comp_comb_type
      :=
@@ -948,8 +892,6 @@ Program Fixpoint FANF (e : @exp 0) (g: isANF e) {measure (esize e)}: anfP e g :=
       | Sig A B iA iB => (fSig A B
                                iA (FANF A (inr (inl iA)))
                                iB (fun x => (FANF (open x B) (inr (inl (open_conf iB))))))
-      | Refl v i => (fRfl v i (FANF v (inl i)))
-      | Eqv v1 v2 i1 i2 => (fEqv v1 v2 i1 (FANF v1 (inl i1)) i2 (FANF v2 (inl i2)))
       end
     | inr (inl ic) =>
       match ic with
@@ -988,8 +930,6 @@ Program Fixpoint FANF (e : @exp 0) (g: isANF e) {measure (esize e)}: anfP e g :=
                       | Sig A B iA iB => (fSig A B
                                                iA (FANF A (inr (inl iA)))
                                                iB (fun x => (FANF (open x B) (inr (inl (open_conf iB))))))
-                      | Refl v i => (fRfl v i (FANF v (inl i)))
-                      | Eqv v1 v2 i1 i2 => (fEqv v1 v2 i1 (FANF v1 (inl i1)) i2 (FANF v2 (inl i2)))
                       end))
                end))
       end
@@ -1019,8 +959,6 @@ Program Fixpoint FANF (e : @exp 0) (g: isANF e) {measure (esize e)}: anfP e g :=
             | Sig A B iA iB => (fSig A B
                                      iA (FANF A (inr (inl iA)))
                                      iB (fun x => (FANF (open x B) (inr (inl (open_conf iB))))))
-            | Refl v i => (fRfl v i (FANF v (inl i)))
-            | Eqv v1 v2 i1 i2 => (fEqv v1 v2 i1 (FANF v1 (inl i1)) i2 (FANF v2 (inl i2)))
             end))
       end
   end.
@@ -1042,7 +980,8 @@ End ANF_val_conf_comp_comb.
 
 Inductive ctxmem :=
 | Assum (A: @exp 0)
-| Def (e: @exp 0) (A: @exp 0).
+| Def (e: @exp 0) (A: @exp 0)
+| Eqv (e1: @exp 0) (e2: @exp 0).
 
 Module envParams <: ContextParams.
   Definition member:= ctxmem.
@@ -1052,6 +991,7 @@ Module envParams <: ContextParams.
   match t with
   | Assum A => Assum ([r] A)
   | Def e A => Def ([r] e) ([r] A)
+  | Eqv e1 e2 => Eqv ([r] e1) ([r] e2)
   end.
   
   Lemma shift_commutes_total: 
